Source/IntegrationTests/TestFiles/LitTests/LitTest/comp/rust/conversions.dfy
@@ -1,0 +1,38 @@
+// NONUNIFORM: Temporary development of the Rust compiler
+// RUN: %baredafny run --target=rs "%s" > "%t"
+// RUN: %diff "%s.expect" "%t"
+
+newtype Uint8 = x: int | 0 <= x < 256
+
+datatype Option<T> = Some(value: T) | None {
+  predicate IsFailure() {
+    None?
+  }
+  function PropagateFailure<U>(): Option<U> {
+    None
+  }
+  function Extract(): T
+    requires !IsFailure() {
+    value
+  }
+  method ExtractMethod() returns (r: T)
+    requires !IsFailure() {
+    return value;
+  }
+}
+
+method TestCompile(input: Option<Uint8>) returns (output: Option<Uint8>) {
+  var middle :- input;
+  var middleMethod := Some(middle).ExtractMethod();
+  return None;
+}
+
+method Main() {
+  var x: Uint8 := 2;
+  // Correct rendering of expressions that can interpret the first '<' as a generic argument
+  var y: bv16 := (x as bv16) << 2;
+  expect y == 8;
+  expect (x as bv16) < 3;
+  expect (x as bv16) <= 3;
+  print "Everything is ok.";
+}
